CircuitCorrectness.v
@@ -1,0 +1,1084 @@
+Require Import
+        SGA.Common SGA.Syntax
+        SGA.Semantics SGA.Circuits.
+
+Require Import Coq.Lists.List.
+Import ListNotations.
+
+Section CompilerCorrectness.
+  Context {var_t reg_t fn_t: Type}.
+  Context {reg_t_eq_dec: EqDec reg_t}.
+
+  Context {R: reg_t -> type}.
+  Context {Sigma: fn_t -> ExternalSignature}.
+  Context {REnv: Env reg_t}.
+  Context (r: REnv.(env_t) R).
+  Context (rc: REnv.(env_t) (fun reg => circuit R Sigma (R reg))).
+  Context (sigma: forall f, Sigma f).
+  Open Scope bool_scope.
+
+  Notation Log := (Log R REnv).
+  Notation circuit := (circuit R Sigma).
+  Notation expr := (expr var_t R Sigma).
+  Notation rule := (rule var_t R Sigma).
+  Notation scheduler := (scheduler var_t R Sigma).
+  Notation rule_circuit := (rule_circuit R Sigma REnv).
+  Notation interp_circuit := (interp_circuit r sigma).
+  Notation interp_circuit' := (interp_circuit' r sigma). (* FIXME *)
+
+  (* Record rwdata_result sz := *)
+  (*   { rread0: option (bits 1); *)
+  (*     rread1: option (bits 1); *)
+  (*     rwrite0: option (bits 1); *)
+  (*     rwrite1: option (bits 1); *)
+  (*     rdata0: option (bits sz); *)
+  (*     rdata1: option (bits sz) }. *)
+
+  Record rwdata_result sz :=
+    { rread0: bits 1;
+      rread1: bits 1;
+      rwrite0: bits 1;
+      rwrite1: bits 1;
+      rdata0: bits sz;
+      rdata1: bits sz }.
+
+  Definition interp_rwdata {sz} (reg: @rwdata reg_t fn_t R Sigma sz) :=
+    {| rread0 := interp_circuit' reg.(read0);
+       rread1 := interp_circuit' reg.(read1);
+       rwrite0 := interp_circuit' reg.(write0);
+       rwrite1 := interp_circuit' reg.(write1);
+       rdata0 := interp_circuit' reg.(data0);
+       rdata1 := interp_circuit' reg.(data1) |}.
+
+  Definition rwdata_of_log (l: Log) : REnv.(env_t) (fun idx => rwdata_result (R idx)).
+  Admitted.
+
+  Definition log_rwdata_consistent l r :=
+    rwdata_of_log l =
+    REnv.(Environments.map) (fun idx v => interp_rwdata v) r.
+
+  (* Lemma canFire_expr_increasing {nRegs}: *)
+  (*   forall {sig} (rl: rule sig) cLog (c1 c2: rule_circuit), *)
+  (*     interp_circuit (willFire_of_canFire c1 cLog) = w1 false -> *)
+  (*     compile_rule v cLog Gamma r c1 = Some c2 -> *)
+  (*     interp_circuit (willFire_of_canFire c2 cLog) = w1 false. *)
+  (* Proof. *)
+  (* Admitted. *)
+
+  (* Lemma canFire_rule_increasing {nRegs}: *)
+  (*   forall {sig} (rl: rule sig) cLog (c1 c2: rule_circuit), *)
+  (*     interp_circuit (willFire_of_canFire c1 cLog) = w1 false -> *)
+  (*     compile_rule v cLog Gamma r c1 = Some c2 -> *)
+  (*     interp_circuit (willFire_of_canFire c2 cLog) = w1 false. *)
+  (* Proof. *)
+  (* Admitted. *)
+
+  (* Context (Gamma: vcontext sig). *)
+  (* Definition gamma_consistent (gamma: gammaEnv.(env_t)) (Gamma: GammaEnv.(env_t)) := *)
+  (*   (forall k c, getenv gamma k = Some c -> exists v, getenv Gamma k = Some v) /\ *)
+  (*   (forall k v, getenv Gamma k = Some v -> exists c, getenv gamma k = Some c) /\ *)
+  (*   (forall k c v, getenv Gamma k = Some v -> getenv gamma k = Some c -> retVal_consistent v (interp_circuit c)). *)
+
+  (* Lemma gamma_consistent_putenv (gamma: gammaEnv.(env_t)) (Gamma: GammaEnv.(env_t)) : *)
+  (*   forall k v c, *)
+  (*     gamma_consistent gamma Gamma -> *)
+  (*     retVal_consistent v (interp_circuit c) -> *)
+  (*     gamma_consistent (putenv gamma k c) (putenv Gamma k v). *)
+  (* Proof. *)
+  (* Admitted. *)
+
+  (* Hint Resolve gamma_consistent_putenv : circuits. *)
+  (* Hint Resolve canFire_increasing : circuits. *)
+
+  Ltac ceauto :=
+    eauto with circuits.
+
+  Definition bool_lt b1 b2 :=
+    b2 = false ->
+    b1 = false.
+
+  Lemma bool_lt_impl b1 b2 :
+    bool_lt b1 b2 <-> (orb (negb b1) b2) = true.
+  Proof.
+    destruct b1, b2; unfold bool_lt; cbn; intuition.
+  Qed.
+
+  Definition circuit_lt (c1 c2: circuit 1) :=
+    bool_lt (Bits.single (interp_circuit' c1)) (Bits.single (interp_circuit' c2)).
+
+  Lemma interp_circuit_circuit_lt_helper_false :
+    forall c1 c2,
+      circuit_lt c1 c2 ->
+      interp_circuit' c2 = Ob~0 ->
+      interp_circuit' c1 = Ob~0.
+  Proof.
+    unfold circuit_lt; intros * Hlt Heq;
+      destruct (interp_circuit' c1) as (? & [ ]), (interp_circuit' c2) as (? & []).
+    inversion Heq; cbv; f_equal; apply Hlt; cbn; congruence.
+  Qed.
+
+  Lemma interp_circuit_circuit_lt_helper_true :
+    forall c1 c2,
+      circuit_lt c1 c2 ->
+      interp_circuit' c1 = Ob~1 ->
+      interp_circuit' c2 = Ob~1.
+  Proof.
+    unfold circuit_lt; intros * Hlt Heq;
+      destruct (interp_circuit' c1) as (? & [ ]), (interp_circuit' c2) as ([ | ] & []);
+      inversion Heq; subst; intuition.
+  Qed.
+
+  Lemma circuit_lt_CAnnot_l :
+    forall s c1 c2,
+      circuit_lt c1 c2 ->
+      circuit_lt (CAnnot s c1) c2.
+  Proof. firstorder. Qed.
+
+  Lemma circuit_lt_CAnnot_r :
+    forall s c1 c2,
+      circuit_lt c1 c2 ->
+      circuit_lt c1 (CAnnot s c2).
+  Proof. firstorder. Qed.
+
+  Lemma bool_lt_and :
+    forall b1 b1' b2 b2',
+      bool_lt b1 b1' ->
+      bool_lt b2 b2' ->
+      bool_lt (andb b1 b2) (andb b1' b2').
+  Proof.
+    unfold bool_lt; intros.
+    destruct b1, b2, b1', b2'; cbn;
+      intuition discriminate.
+  Qed.
+
+  Lemma bool_lt_and_l :
+    forall b1 b1' b2,
+      bool_lt b1 b1' ->
+      bool_lt (andb b1 b2) b1'.
+  Proof.
+    unfold bool_lt; intros.
+    destruct b1, b2, b1'; cbn;
+      intuition discriminate.
+  Qed.
+
+  Lemma bool_lt_or :
+    forall b1 b1' b2 b2',
+      bool_lt b1 b1' ->
+      bool_lt b2 b2' ->
+      bool_lt (orb b1 b2) (orb b1' b2').
+  Proof.
+    unfold bool_lt; intros.
+    destruct b1, b2, b1', b2'; cbn;
+      intuition discriminate.
+  Qed.
+
+  Lemma bool_lt_mux :
+    forall (s: bool) b1 b1' b2 b2',
+      bool_lt b1 b1' ->
+      bool_lt b2 b2' ->
+      bool_lt (if s then b1 else b2) (if s then b1' else b2').
+  Proof.
+    unfold bool_lt; intros.
+    destruct s; cbn;
+      intuition discriminate.
+  Qed.
+
+  Lemma bool_lt_not :
+    forall b1 b2,
+      bool_lt b1 b2 ->
+      bool_lt (negb b2) (negb b1).
+  Proof.
+    unfold bool_lt; intros.
+    destruct b1, b2; cbn;
+      intuition discriminate.
+  Qed.
+
+  Lemma bool_lt_true :
+    forall b, bool_lt b true.
+  Proof.
+    unfold bool_lt; intros;
+      destruct b; intuition discriminate.
+  Qed.
+
+  Lemma bool_lt_false :
+    forall b, bool_lt false b.
+  Proof.
+    unfold bool_lt; intros;
+      destruct b; intuition discriminate.
+  Qed.
+
+  Lemma circuit_lt_CAnd :
+    forall c1 c1' c2 c2',
+      circuit_lt c1 c1' ->
+      circuit_lt c2 c2' ->
+      circuit_lt (CAnd c1 c2) (CAnd c1' c2').
+  Proof. unfold circuit_lt; cbn; eauto using bool_lt_and. Qed.
+
+  Lemma circuit_lt_CAnd_l :
+    forall c1 c1' c2,
+      circuit_lt c1 c1' ->
+      circuit_lt (CAnd c1 c2) c1'.
+  Proof. unfold circuit_lt; cbn; eauto using bool_lt_and_l. Qed.
+
+  Lemma circuit_lt_CAnd_r :
+    forall c1 c1' c2',
+      circuit_lt c1 c1' ->
+      interp_circuit' c2' = Ob~1 ->
+      circuit_lt c1 (CAnd c1' c2').
+  Proof. unfold circuit_lt; cbn. intros * ? ->.
+     cbn; rewrite Bool.andb_true_r; eauto. Qed.
+
+  Lemma circuit_lt_COr :
+    forall c1 c1' c2 c2',
+      circuit_lt c1 c1' ->
+      circuit_lt c2 c2' ->
+      circuit_lt (COr c1 c2) (COr c1' c2').
+  Proof. unfold circuit_lt; cbn; eauto using bool_lt_or. Qed.
+
+  Lemma circuit_lt_CMux :
+    forall s c1 c1' c2 c2',
+      circuit_lt c1 c1' ->
+      circuit_lt c2 c2' ->
+      circuit_lt (CMux s c1 c2) (CMux s c1' c2').
+  Proof.
+    unfold circuit_lt; cbn;
+      intros; destruct (Bits.single (interp_circuit' s)); eauto.
+  Qed.
+
+  Lemma circuit_lt_CMux_l :
+    forall s c1 c2 c3,
+      (interp_circuit' s = Ob~1 -> circuit_lt c1 c3) ->
+      (interp_circuit' s = Ob~0 -> circuit_lt c2 c3) ->
+      circuit_lt (CMux s c1 c2) c3.
+  Proof.
+    unfold circuit_lt; cbn;
+      intros * Heq1 Heq2; destruct (interp_circuit' s) as [ b [] ]; cbn.
+    destruct b; eauto.
+  Qed.
+
+  Lemma circuit_lt_CMux_r :
+    forall s c1 c2 c3,
+      (interp_circuit' s = Ob~1 -> circuit_lt c1 c2) ->
+      (interp_circuit' s = Ob~0 -> circuit_lt c1 c3) ->
+      circuit_lt c1 (CMux s c2 c3).
+  Proof.
+    unfold circuit_lt; cbn;
+      intros * Heq1 Heq2; destruct (interp_circuit' s) as [ b [] ]; cbn.
+    destruct b; eauto.
+  Qed.
+
+  Lemma circuit_lt_CNot :
+    forall c1 c2,
+      circuit_lt c1 c2 ->
+      circuit_lt (CNot c2) (CNot c1).
+  Proof. unfold circuit_lt; cbn; eauto using bool_lt_not. Qed.
+
+  Lemma circuit_lt_true :
+    forall c, circuit_lt c (CConst Ob~1).
+  Proof. unfold circuit_lt; cbn; eauto using bool_lt_true. Qed.
+
+  Lemma circuit_lt_false :
+    forall c, circuit_lt (CConst Ob~0) c.
+  Proof. unfold circuit_lt; cbn; eauto using bool_lt_false. Qed.
+
+  Lemma circuit_lt_fold_right {X} :
+    forall (xs: list X) f0 f1 c0 c1,
+      circuit_lt c1 c0 ->
+      (forall x acc1 acc0, circuit_lt acc1 acc0 -> circuit_lt (f1 x acc1) (f0 x acc0)) ->
+      circuit_lt (List.fold_right f1 c1 xs) (List.fold_right f0 c0 xs).
+  Proof.
+    induction xs; cbn; intros * Hlt Hxlt; eauto.
+  Qed.
+
+  Lemma circuit_lt_refl :
+    forall c, circuit_lt c c.
+  Proof. firstorder. Qed.
+
+  Lemma circuit_lt_trans :
+    forall c1 c2 c3,
+      circuit_lt c1 c2 ->
+      circuit_lt c2 c3 ->
+      circuit_lt c1 c3.
+  Proof. firstorder. Qed.
+
+  Lemma circuit_lt_willFire_of_canFire_canFire :
+    forall c1 (cLog: scheduler_circuit R Sigma REnv) rws,
+      circuit_lt (willFire_of_canFire {| canFire := c1; regs := rws |} cLog) c1.
+  Proof.
+    unfold willFire_of_canFire; intros.
+    eapply circuit_lt_trans.
+    - eapply circuit_lt_fold_right.
+      + apply circuit_lt_refl.
+      + intros; rewrite !getenv_zip.
+        eapply circuit_lt_CAnd.
+        * eassumption.
+        * apply circuit_lt_true.
+    - cbn.
+      induction finite_elems; cbn.
+      + apply circuit_lt_refl.
+      + apply circuit_lt_CAnd_l; eassumption.
+  Qed.
+
+  Definition rwdata_circuit_lt_invariant {idx} (rwd1 rwd2: rwdata R Sigma (R idx)) :=
+      circuit_lt (rwd1.(read0)) (rwd2.(read0)) /\
+      circuit_lt (rwd1.(write0)) (rwd2.(write0)) /\
+      circuit_lt (rwd1.(read1)) (rwd2.(read1)) /\
+      circuit_lt (rwd1.(write1)) (rwd2.(write1)).
+
+  Definition rwset_circuit_lt_invariant (rws1 rws2: rwset) idx :=
+    rwdata_circuit_lt_invariant
+      (REnv.(getenv) rws1 idx)
+      (REnv.(getenv) rws2 idx).
+
+  Lemma rwset_circuit_lt_invariant_refl :
+    forall rws idx, rwset_circuit_lt_invariant rws rws idx.
+  Proof. firstorder using circuit_lt_refl. Qed.
+
+  Lemma rwset_circuit_lt_invariant_trans :
+    forall rws1 rws2 rws3 idx,
+      rwset_circuit_lt_invariant rws1 rws2 idx ->
+      rwset_circuit_lt_invariant rws2 rws3 idx ->
+      rwset_circuit_lt_invariant rws1 rws3 idx.
+  Proof. firstorder using circuit_lt_trans. Qed.
+
+
+  Lemma rwset_circuit_lt_invariant_putenv_eq :
+    forall rws1 rws2 idx rwd0,
+    rwdata_circuit_lt_invariant (REnv.(getenv) rws1 idx) rwd0 ->
+    rwset_circuit_lt_invariant rws1 (REnv.(putenv) rws2 idx rwd0) idx.
+  Proof.
+    unfold rwset_circuit_lt_invariant; intros.
+    rewrite get_put_eq; eauto.
+  Qed.
+
+  Lemma rwset_circuit_lt_invariant_putenv_neq :
+    forall rws1 rws2 idx idx0 rwd0,
+      idx <> idx0 ->
+      rwset_circuit_lt_invariant rws1 rws2 idx ->
+      rwset_circuit_lt_invariant rws1 (REnv.(putenv) rws2 idx0 rwd0) idx.
+  Proof.
+    unfold rwset_circuit_lt_invariant; intros.
+    rewrite get_put_neq; eauto.
+  Qed.
+
+  Lemma rwset_circuit_lt_invariant_putenv :
+    forall rws1 rws2 idx0 rwd0,
+      (forall idx, rwset_circuit_lt_invariant rws1 rws2 idx) ->
+      rwdata_circuit_lt_invariant (getenv REnv rws1 idx0) rwd0 ->
+      (forall idx, rwset_circuit_lt_invariant rws1 (REnv.(putenv) rws2 idx0 rwd0) idx).
+  Proof.
+    intros.
+    destruct (eq_dec idx0 idx); subst;
+      eauto using rwset_circuit_lt_invariant_putenv_eq, rwset_circuit_lt_invariant_putenv_neq.
+  Qed.
+
+  Lemma rwdata_circuit_lt_invariant_mux_rwdata_l :
+    forall c idx rwd1 rwd2 rwd3,
+      (interp_circuit' c = Ob~1 -> @rwdata_circuit_lt_invariant idx rwd1 rwd3) ->
+      (interp_circuit' c = Ob~0 -> @rwdata_circuit_lt_invariant idx rwd2 rwd3) ->
+      @rwdata_circuit_lt_invariant idx (mux_rwdata c rwd1 rwd2) rwd3.
+  Proof.
+    unfold rwdata_circuit_lt_invariant, mux_rwdata; cbn; intros.
+    repeat split; apply circuit_lt_CMux_l; intuition eauto.
+  Qed.
+
+  Lemma rwdata_circuit_lt_invariant_mux_rwdata_r :
+    forall c idx rwd1 rwd2 rwd3,
+      (interp_circuit' c = Ob~1 -> @rwdata_circuit_lt_invariant idx rwd1 rwd2) ->
+      (interp_circuit' c = Ob~0 -> @rwdata_circuit_lt_invariant idx rwd1 rwd3) ->
+      @rwdata_circuit_lt_invariant idx rwd1 (mux_rwdata c rwd2 rwd3).
+  Proof.
+    unfold rwdata_circuit_lt_invariant, mux_rwdata; cbn; intros.
+    repeat split; apply circuit_lt_CMux_r; intuition eauto.
+  Qed.
+
+  Lemma rwset_circuit_lt_compile_expr_correct {sig tau} :
+    forall (gamma : ccontext sig) (ex : expr sig tau) (rwc : rwcircuit),
+      circuit_lt (canFire (erwc (compile_expr rc gamma ex rwc))) (canFire rwc) /\
+      forall idx, rwset_circuit_lt_invariant (rwc.(regs)) ((compile_expr rc gamma ex rwc).(erwc).(regs)) idx.
+  Proof.
+    induction ex; cbn; intros; eauto using circuit_lt_refl, rwset_circuit_lt_invariant_refl.
+    - destruct port; cbn.
+      (* Read0 *)
+      + split.
+        * apply circuit_lt_CAnnot_l, circuit_lt_CAnd_l, circuit_lt_refl.
+        * intros. eapply rwset_circuit_lt_invariant_putenv.
+          -- eauto using rwset_circuit_lt_invariant_refl.
+          -- red; cbn; eauto using circuit_lt_true, circuit_lt_refl.
+      (* Read1 *)
+      + split.
+        * eauto using circuit_lt_refl.
+        * intros; apply rwset_circuit_lt_invariant_putenv.
+          -- eauto using rwset_circuit_lt_invariant_refl.
+          -- red; cbn; eauto using circuit_lt_true, circuit_lt_refl.
+    - specialize (IHex1 rwc);
+        specialize (IHex2 (erwc (compile_expr rc gamma ex1 rwc))).
+      intuition eauto using circuit_lt_trans, rwset_circuit_lt_invariant_trans.
+  Qed.
+
+  Ltac circuit_lt_f_equal :=
+    repeat (apply circuit_lt_CAnnot_l ||
+            apply circuit_lt_CAnnot_r ||
+            apply circuit_lt_CAnd ||
+            apply circuit_lt_COr ||
+            apply circuit_lt_CNot ||
+            apply circuit_lt_true ||
+            apply circuit_lt_false ||
+            apply circuit_lt_refl).
+
+  Lemma rwset_circuit_lt_compile_rule_correct {sig}:
+    forall (rl : rule sig) (gamma : ccontext sig) (rwc : rwcircuit),
+      circuit_lt (canFire (compile_rule rc gamma rl rwc)) (canFire rwc) /\
+      forall idx, rwset_circuit_lt_invariant (rwc.(regs)) ((compile_rule rc gamma rl rwc).(regs)) idx.
+  Proof.
+    induction rl; cbn; intros;
+      try solve [split; circuit_lt_f_equal; eauto using rwset_circuit_lt_invariant_refl].
+    - (* Seq *)
+      specialize (IHrl1 gamma rwc);
+        specialize (IHrl2 gamma (compile_rule rc gamma rl1 rwc)).
+      intuition eauto using circuit_lt_trans, rwset_circuit_lt_invariant_trans.
+    - (* Bind *)
+      pose proof (rwset_circuit_lt_compile_expr_correct gamma ex rwc).
+      specialize (IHrl (CtxCons (var, tau) (retVal (compile_expr rc gamma ex rwc)) gamma)
+                       (erwc (compile_expr rc gamma ex rwc))).
+      intuition eauto using circuit_lt_trans, rwset_circuit_lt_invariant_trans.
+    - (* If *)
+      pose proof (rwset_circuit_lt_compile_expr_correct gamma cond rwc).
+      specialize (IHrl1 gamma (erwc (compile_expr rc gamma cond rwc))).
+      specialize (IHrl2 gamma (erwc (compile_expr rc gamma cond rwc))).
+      split.
+      + circuit_lt_f_equal.
+        apply circuit_lt_CMux_l;
+          intuition eauto using circuit_lt_trans, rwset_circuit_lt_invariant_trans.
+      + unfold map2; red; intros.
+        rewrite getenv_create.
+        apply rwdata_circuit_lt_invariant_mux_rwdata_r;
+          intros; eapply rwset_circuit_lt_invariant_trans; intuition eauto.
+    - (* Write *)
+      pose proof (rwset_circuit_lt_compile_expr_correct gamma value rwc) as (Hpr & Hpr').
+      (* destruct port; cbn. *)
+      + split.
+        * destruct port;
+            circuit_lt_f_equal;
+            apply circuit_lt_CAnd_l;
+            intuition.
+        * intros; destruct port;
+            (apply rwset_circuit_lt_invariant_putenv;
+             [ | specialize (Hpr' idx); red in Hpr' |- *; red in Hpr'; cbn;
+                 repeat cleanup_step ];
+             intuition eauto using circuit_lt_true).
+  Qed.
+
+  Lemma expr_compile_willFire_of_canFire'_decreasing {sig}:
+    forall t (ex : expr sig t) (gamma : ccontext sig) (rwc : rwcircuit) idx rwd,
+      circuit_lt (willFire_of_canFire' (getenv REnv (regs (erwc (compile_expr rc gamma ex rwc))) idx) rwd)
+                 (willFire_of_canFire' (getenv REnv (regs rwc) idx) rwd).
+  Proof.
+    unfold willFire_of_canFire'; intros.
+    pose proof (rwset_circuit_lt_compile_expr_correct gamma ex rwc) as (HCanfire & Hc);
+      specialize (Hc idx); red in Hc; red in Hc; repeat cleanup_step.
+    circuit_lt_f_equal; eauto.
+  Qed.
+
+  Lemma rule_compile_willFire_of_canFire'_decreasing {sig}:
+    forall (rl : rule sig) (gamma : ccontext sig) (rwc : rwcircuit) idx rwd,
+      circuit_lt (willFire_of_canFire' (getenv REnv (regs (compile_rule rc gamma rl rwc)) idx) rwd)
+                 (willFire_of_canFire' (getenv REnv (regs rwc) idx) rwd).
+  Proof.
+    unfold willFire_of_canFire'; intros.
+    pose proof (rwset_circuit_lt_compile_rule_correct rl gamma rwc) as (HCanfire & Hc);
+      specialize (Hc idx); red in Hc; red in Hc; repeat cleanup_step.
+    circuit_lt_f_equal; eauto.
+  Qed.
+
+  Lemma expr_compile_willFire_of_canFire_decreasing {sig}:
+    forall t (ex : expr sig t) (cLog : scheduler_circuit R Sigma REnv)
+      (gamma : ccontext sig) (rwc : rwcircuit),
+      circuit_lt (willFire_of_canFire (erwc (compile_expr rc gamma ex rwc)) cLog)
+                 (willFire_of_canFire rwc cLog).
+  Proof.
+    intros.
+    unfold willFire_of_canFire.
+    unfold Environments.fold_right.
+    eapply circuit_lt_fold_right.
+    - pose proof (rwset_circuit_lt_compile_expr_correct gamma ex rwc); intuition.
+    - intros; cbn.
+      rewrite !getenv_zip.
+      apply circuit_lt_CAnnot_l, circuit_lt_CAnnot_r, circuit_lt_CAnd.
+      + eassumption.
+      + eauto using expr_compile_willFire_of_canFire'_decreasing.
+  Qed.
+
+  Lemma rule_compile_willFire_of_canFire_decreasing {sig}:
+    forall (rl : rule sig) (cLog : scheduler_circuit R Sigma REnv)
+      (gamma : ccontext sig) (rwc : rwcircuit),
+      circuit_lt (willFire_of_canFire (compile_rule rc gamma rl rwc) cLog)
+                 (willFire_of_canFire rwc cLog).
+  Proof.
+    intros.
+    unfold willFire_of_canFire.
+    unfold Environments.fold_right.
+    eapply circuit_lt_fold_right.
+    - pose proof (rwset_circuit_lt_compile_rule_correct rl gamma rwc); intuition.
+    - intros; cbn.
+      rewrite !getenv_zip.
+      apply circuit_lt_CAnnot_l, circuit_lt_CAnnot_r, circuit_lt_CAnd.
+      + eassumption.
+      + eauto using rule_compile_willFire_of_canFire'_decreasing.
+  Qed.
+
+  Lemma willFire_of_canFire_decreasing :
+    forall c1 c2 (cLog: scheduler_circuit R Sigma REnv) rws,
+      circuit_lt c1 c2 ->
+      circuit_lt (willFire_of_canFire {| canFire := c1; regs := rws |} cLog)
+                 (willFire_of_canFire {| canFire := c2; regs := rws |} cLog).
+  Proof.
+    unfold willFire_of_canFire; intros.
+    eapply circuit_lt_fold_right.
+    - eassumption.
+    - intros; rewrite !getenv_zip.
+      cbn.
+      eauto using circuit_lt_CAnnot_l, circuit_lt_CAnd, circuit_lt_refl.
+  Qed.
+
+  Ltac t_step :=
+    match goal with
+    | _ => cleanup_step
+    | _ => progress intros
+    | [ Heq: interp_circuit ?x = Some _ |- context[interp_circuit ?x] ] =>
+      rewrite Heq
+    | [ IH: context[interp_expr _ _ _ _ _ ?ex] |-
+        context[interp_expr _ _ ?Gamma ?Log ?log ?ex] ] =>
+      specialize (IH _ Gamma _ log ltac:(eauto) ltac:(eauto) ltac:(eauto) ltac:(eauto));
+      cbv zeta in IH;
+      destruct (interp_expr _ _ Gamma Log log ex) as [(? & ?) | ] eqn:?; cbn
+    | [ |- match (if ?x then _ else _) with _ => _ end ] =>
+      destruct x eqn:?; cbn
+    | [ IH: context[interp_rule _ _ _ _ _ ?rl] |-
+        context[interp_rule _ _ ?Gamma ?Log ?log ?rl] ] =>
+      specialize (IH _ Gamma _ log ltac:(eauto) ltac:(eauto) ltac:(eauto) ltac:(eauto));
+      cbv zeta in IH;
+      destruct (interp_rule _ _ Gamma Log log rl) as [? | ] eqn:?; cbn
+    end.
+
+  (* Create HintDb circuits discriminated. *)
+  Ltac t := repeat t_step; eauto.  (* with circuits. *)
+
+  Require Import Bool.
+  (* https://coq-club.inria.narkive.com/HeWqgvKm/boolean-simplification *)
+  Hint Rewrite
+       orb_false_r (** b || false -> b *)
+       orb_false_l (** false || b -> b *)
+       orb_true_r (** b || true -> true *)
+       orb_true_l (** true || b -> true *)
+       andb_false_r (** b && false -> false *)
+       andb_false_l (** false && b -> false *)
+       andb_true_r (** b && true -> b *)
+       andb_true_l (** true && b -> b *)
+       negb_orb (** negb (b || c) -> negb b && negb c *)
+       negb_andb (** negb (b && c) -> negb b || negb c *)
+       negb_involutive (** negb( (negb b) -> b *)
+    : bool_simpl.
+  Ltac bool_simpl := autorewrite with bool_simpl in *.
+
+  Lemma expr_compiler_correct {sig tau} Log cLog:
+    forall (ex: expr sig tau) (clog: rule_circuit)
+      (Gamma: vcontext sig) (gamma: ccontext sig) log,
+      log_rwdata_consistent log clog.(regs) ->
+      (forall k tau' (m: member (k, tau') sig) , interp_circuit' (cassoc m gamma) = cassoc m Gamma) ->
+      (forall idx, interp_circuit' (getenv REnv rc idx) = getenv REnv r idx) ->
+      interp_circuit' (willFire_of_canFire clog cLog) = Ob~1 ->
+      let cExpr := compile_expr rc gamma ex clog in
+      match interp_expr r sigma Gamma Log log ex with
+      | Some (l', v) =>
+        interp_circuit' cExpr.(retVal) = v /\
+        log_rwdata_consistent l' cExpr.(erwc).(regs) /\
+        interp_circuit' (willFire_of_canFire cExpr.(erwc) cLog) = Ob~1
+      | None =>
+        interp_circuit' (willFire_of_canFire cExpr.(erwc) cLog) = Ob~0
+      end.
+  Proof.
+    induction ex; intros.
+    - (* Var *) cbn; eauto.
+    - (* Const *) cbn; eauto.
+    - (* Read *)
+      destruct port.
+      + cbn.
+        destruct (may_read0 Log log idx) eqn:?; cbn.
+        * repeat split.
+          -- eauto.
+          -- admit.
+          -- eapply interp_circuit_circuit_lt_helper_true; try eassumption.
+             unfold willFire_of_canFire, willFire_of_canFire'; cbn.
+             apply circuit_lt_fold_right.
+             ++ apply circuit_lt_CAnd_r.
+                apply circuit_lt_refl.
+                cbn. admit.
+             ++ intros.
+                rewrite !getenv_zip; cbn.
+                destruct (eq_dec idx x); subst;
+                  [ rewrite !get_put_eq | rewrite !get_put_neq by eassumption ];
+                  cbn;
+                  circuit_lt_f_equal;
+                  try eassumption.
+                unfold circuit_lt; cbn.
+                apply bool_lt_impl.
+                replace (interp_circuit' (write0 (getenv REnv (sregs cLog) x))) with Ob~0 by admit.
+                replace (interp_circuit' (write1 (getenv REnv (sregs cLog) x))) with Ob~0 by admit.
+                cbn; bool_simpl; reflexivity.
+        * eapply interp_circuit_circuit_lt_helper_false.
+          apply circuit_lt_willFire_of_canFire_canFire.
+          cbn.
+          cut ((interp_circuit' (read1 (getenv REnv (regs clog) idx))) = Ob~1 \/
+               (interp_circuit' (write1 (getenv REnv (regs clog) idx))) = Ob~1).
+          intros [-> | ->]; bool_simpl; reflexivity.
+          admit.
+      + cbn.
+        destruct (may_read1 Log idx) eqn:?; cbn.
+        * repeat split.
+          -- admit. (* Log consistency property *)
+          -- admit.
+          -- eapply interp_circuit_circuit_lt_helper_true; try eassumption.
+             unfold willFire_of_canFire, willFire_of_canFire'; cbn.
+             apply circuit_lt_fold_right.
+             ++ circuit_lt_f_equal.
+             ++ intros.
+                rewrite !getenv_zip; cbn.
+                destruct (eq_dec idx x); subst;
+                  [ rewrite !get_put_eq | rewrite !get_put_neq by eassumption ];
+                  cbn;
+                  circuit_lt_f_equal;
+                  try eassumption.
+                unfold circuit_lt; cbn.
+                apply bool_lt_impl.
+                replace (interp_circuit' (write1 (getenv REnv (sregs cLog) x))) with Ob~0 by admit.
+                cbn; bool_simpl; reflexivity.
+        * (* FIXME write two lemmas to focus on the changed element in regs *)
+          admit. (* may_read1 = false -> there's a write1 *)
+    - (* Call *)
+      repeat t_step; eauto.
+      eapply interp_circuit_circuit_lt_helper_false;
+        eauto using expr_compile_willFire_of_canFire_decreasing.
+  Admitted.
+
+  Lemma rule_compiler_correct {sig} Log cLog:
+    forall (rl: rule sig) (clog: rule_circuit)
+      (Gamma: vcontext sig) (gamma: ccontext sig) log,
+      log_rwdata_consistent log clog.(regs) ->
+      (forall k tau' (m: member (k, tau') sig) , interp_circuit' (cassoc m gamma) = cassoc m Gamma) ->
+      (forall idx, interp_circuit' (getenv REnv rc idx) = (getenv REnv r idx)) ->
+      interp_circuit' (willFire_of_canFire clog cLog) = Ob~1 ->
+      let cRule := compile_rule rc gamma rl clog in
+      match interp_rule r sigma Gamma Log log rl with
+      | Some (l') =>
+        log_rwdata_consistent l' cRule.(regs) /\
+        interp_circuit' (willFire_of_canFire cRule cLog) = Ob~1
+      | None =>
+        interp_circuit' (willFire_of_canFire cRule cLog) = Ob~0
+      end.
+  Proof.
+    induction rl; intros; try solve[cbn; eauto].
+    - (* Fail *)
+      cbn; intros.
+      destruct clog.
+      eapply interp_circuit_circuit_lt_helper.
+      + apply circuit_lt_willFire_of_canFire_canFire.
+      + reflexivity.
+    - (* Seq *)
+      cbn.
+      t.
+      eapply interp_circuit_circuit_lt_helper;
+        eauto using rule_compile_willFire_of_canFire_decreasing.
+    - (* Bind *)
+      cbn.
+      pose proof (@expr_compiler_correct sig tau Log cLog ex).
+      t.
+      + cbn.
+        (* Need lemma to be able to specialize IH despite the CtxCons *)
+        (* lazymatch goal with *)
+        (* | [ IH: context[interp_rule _ _ _ _ _ ?rl] |- *)
+        (*     context[interp_rule _ _ ?Gamma ?Log ?log ?rl] ] => *)
+        (*   specialize (fun cc => IH _ Gamma cc log ltac:(eauto) ltac:(eauto) ltac:(eauto) ltac:(eauto)); *)
+        (*     cbv zeta in IH *)
+        (* end. *)
+        (*     destruct (interp_rule _ _ Gamma Log log rl) as [? | ] eqn:?; cbn *)
+        (*             end. *)
+        admit.
+      + eapply interp_circuit_circuit_lt_helper;
+          eauto using rule_compile_willFire_of_canFire_decreasing.
+    - (* If *)
+      pose proof (@expr_compiler_correct sig _ Log cLog cond).
+      cbn; t.
+      + split.
+        admit.
+        
+      + destruct (Bits.single _); cbn.
+        admit.                    (* WF_cF and mux lemmas *)
+        admit.                    (* WF_cF and mux lemmas *)
+      + admit. (* More WF decreasing, but with cmux this time. *)
+    - (* Write *)
+      cbn.
+      t.
+      pose proof (@expr_compiler_correct sig _ Log cLog value).
+      t.
+      + destruct (may_write Log l port idx); cbn.
+        * admit.
+        * admit. (* decreasing *)
+      + admit. (* decreasing *)
+  Admitted.
+
+  Lemma scheduler_compiler_correct:
+    forall (s: scheduler) Log cLog,
+      log_rwdata_consistent Log cLog.(sregs) ->
+      (forall idx, interp_circuit (getenv REnv rc idx) = Some (getenv REnv r idx)) ->
+      log_rwdata_consistent
+        (interp_scheduler' r sigma Log s)
+        (compile_scheduler' rc s cLog).(sregs).
+  Proof.
+    induction s; cbn; intros.
+    - eauto.
+    - pose proof (@rule_compiler_correct nil Log cLog r0).
+      unshelve eassert (H1 := H1 _ CtxEmpty _ log_empty ltac:(eauto) ltac:(eauto) ltac:(eauto) ltac:(eauto)).
+      apply CtxEmpty.
+      apply (adapter cLog).     (* Should get these from call to compile_rule *)
+      cbv zeta in H1.
+      destruct (interp_rule r sigma CtxEmpty Log log_empty r0); cbn; t.
+      + set (fun _ => _).
+        set (fun _ => _).
+        set (fun _ => _).
+        admit.                  (* CMuxes simplify because rule doesn't run *)
+      + admit.
+  Admitted.
+      
+      
+lazymatch goal with
+      | [ IH: context[interp_rule _ _ _ _ _ ?rl] |-
+          context[interp_rule _ _ ?Gamma ?Log ?log ?rl] ] =>
+        specialize (IH _ Gamma _ log ltac:(eauto) ltac:(eauto) ltac:(eauto) ltac:(eauto));
+          cbv zeta in IH;
+          destruct (interp_rule _ _ Gamma Log log rl) as [? | ] eqn:?; cbn
+                  end.
+
+      
+  Ltac tstep :=
+      match goal with
+      | _ => cleanup_step
+      | _ => progress intros
+
+      | [ IH: (forall gamma rc, match compile_rule ?sigma ?L gamma ?r rc with _ => _ end)
+          |- match opt_bind (compile_rule ?sigma ?L ?gamma ?r ?rc) _ with _ => _ end] =>
+        specialize (IH gamma rc);
+        destruct (compile_rule sigma L gamma r) eqn:?; cbn; ceauto; []
+
+      | [ IH: (forall Gamma l,
+                  gamma_consistent _ Gamma ->
+                  log_rwdata_consistent l (regs ?rc) ->
+                  interp_circuit (willFire_of_canFire ?rc _) = w1 true ->
+                  match interp_rule ?R ?Sigma Gamma ?L l ?r with _ => _ end)
+          |- context [interp_rule ?R ?Sigma ?Gamma ?L ?l ?r] ] =>
+        specialize (IH Gamma l ltac:(ceauto) ltac:(ceauto) ltac:(ceauto));
+        destruct (interp_rule R Sigma Gamma L l r) as [(? & ?) | | ] eqn:?; cbn
+
+      | [ |- match opt_bind ?x _ with _ => _ end] =>
+        destruct x eqn:?; cbn; ceauto; []
+
+      | [ |- match result_bind (opt_result Stuck ?x) _ with _ => _ end] =>
+        destruct x eqn:?; cbn; ceauto; []
+
+      | [ |- match result_bind (bool_result ?x) _ with _ => _ end] =>
+        destruct x eqn:?; cbn; ceauto; []
+
+      | [ H: getenv ?gamma ?k = Some ?c, H': gamma_consistent ?gamma ?Gamma
+          |- context[getenv ?Gamma ?k] ] =>
+        pose_once (and_fst H') k c H
+
+      | [ |- match (match ?v with _ => _ end) with _ => _ end] =>
+        destruct v eqn:?; cbn; ceauto
+
+      | [ H: retVal_consistent ?v ?bs |- context[?bs] ] =>
+        rewrite H
+
+      | [ H: ?x = ?y |- context[?x] ] =>
+        let y_hd := constr_hd y in
+        is_constructor y_hd; rewrite H
+
+      | [ H: exists _, getenv _ _ = Some _ |- _ ] =>
+        destruct H; try (rewrite H; cbn)
+
+      | [  |- _ /\ _ ] => split
+
+      | _ => progress unfold result_map
+      end.
+
+    Ltac t := repeat tstep; ceauto.
+
+    induction rule; cbn; intros; try solve[t; ceauto].
+
+    Opaque willFire_of_canFire.
+
+    - t.
+
+      + unfold log_rwdata_consistent.
+        intros. erewrite Vector.nth_map2; try reflexivity.
+        unfold interp_rwdata.
+        cbn.
+        t.
+      +
+
+        (* FIXME simplify these cases: in each case the rule is either true or false. *)
+        admit.
+      + unfold log_rwdata_consistent.
+        intros. erewrite Vector.nth_map2; try reflexivity.
+        unfold interp_rwdata.
+        cbn.
+        t.
+      + admit.
+      + unfold log_rwdata_consistent.
+        intros. erewrite Vector.nth_map2; try reflexivity.
+        unfold interp_rwdata.
+        cbn.
+        t.
+      + admit.
+      + admit.
+      + unfold log_rwdata_consistent.
+        intros. erewrite Vector.nth_map2; try reflexivity.
+        unfold interp_rwdata.
+        cbn.
+        t.
+      + admit.
+      + admit.
+      + unfold log_rwdata_consistent.
+        intros. erewrite Vector.nth_map2; try reflexivity.
+        unfold interp_rwdata.
+        cbn.
+        t.
+      + admit.
+      + admit.
+      + admit.
+      + admit.
+      + unfold log_rwdata_consistent.
+        intros. erewrite Vector.nth_map2; try reflexivity.
+        unfold interp_rwdata.
+        cbn.
+        t.
+      + admit.
+      + admit.
+      +
+        Transparent willFire_of_canFire.
+
+Lemma cand_true: forall bs1 bs2,
+          cand bs1 bs2 = w1 true ->
+          bs1 = w1 true /\ bs2 = w1 true.
+        Proof. destruct bs1 as [ | [ | ] [ | ? ] ]; cbn;
+             destruct bs2 as [ | [ | ] [ | ? ] ]; cbn.
+           all: intros; try discriminate; eauto.
+        Qed.
+
+Arguments willFire_of_canFire' : simpl never.
+  Lemma interp_willFire_of_canFire {nRegs}:
+    forall cRule cInput,
+      (interp_circuit (cRule.(canFire)) = w1 true /\
+       Vector.Forall2 (fun ruleReg inReg =>
+                         interp_circuit (willFire_of_canFire' ruleReg inReg) = w1 true)
+                      cRule.(regs) cInput.(sregs)) <->
+      interp_circuit (willFire_of_canFire (nRegs := nRegs) cRule cInput) = w1 true.
+  Proof.
+    destruct cRule, cInput; unfold rwset in *; clear R.
+    revert canFire.
+    cbn.
+    pattern regs, sregs.
+    revert regs sregs; revert nRegs.
+    eapply VectorDef.rect2; cbn.
+    - split; [intros (Heq & HForall) | split].
+      + eauto.
+      + eauto.
+      + econstructor.
+    - split; [intros (Heq & HForall) | ].
+      + inversion HForall; subst.
+        rewrite (and_fst (H canFire)), H4.
+        * reflexivity.
+        * Require Import Program.
+          repeat simpl_existT; subst.         (* FIXME use decidable eq instead *)
+          eauto.
+      + intros H0.
+        apply cand_true in H0; destruct H0.
+        rewrite <- H in H0; destruct H0.
+        split.
+        * eauto.
+        * econstructor; eauto.
+  Qed.
+
+  Lemma interp_willFire_of_canFire_false {nRegs}:
+    forall cRule cInput,
+      (interp_circuit (cRule.(canFire)) = w1 false \/
+       Vector.Exists2 (fun ruleReg inReg =>
+                         interp_circuit (willFire_of_canFire' ruleReg inReg) = w1 false)
+                      cRule.(regs) cInput.(sregs)) <->
+      interp_circuit (willFire_of_canFire (nRegs := nRegs) cRule cInput) = w1 false.
+  Proof.
+    destruct cRule, cInput; unfold rwset in *; clear R.
+    revert canFire.
+    cbn.
+    pattern regs, sregs.
+    revert regs sregs; revert nRegs.
+    eapply VectorDef.rect2.
+    - split; [intros [ Heq | HExists ] | intros ].
+      + eauto.
+      + inversion HExists.
+      + eauto.
+    - cbn; split; [intros  [ Heq | HExists ] | intros ].
+      + rewrite (and_fst (H canFire)).
+      (* Needs well-formedness to apply theorem *)
+      + inversion HForall; subst.
+        rewrite (and_fst (H canFire)), H4.
+        * reflexivity.
+        * Require Import Program.
+          repeat simpl_existT; subst.         (* FIXME use decidable eq instead *)
+          eauto.
+      + intros H0.
+        apply cand_true in H0; destruct H0.
+        rewrite <- H in H0; destruct H0.
+        split.
+        * eauto.
+        * econstructor; eauto.
+  Qed.
+
+  
+  
+        
+                                        destruct bs
+    
+    revert dependent nRegs.
+        
+  
+        
+        unfold willFire_of_canFire.
+        cbn.
+
+        admit.
+
+    (* FIMXE handle above admits with setoid rewriting? *)
+    (* Better: prove that interp of fold_left2 is the same as forall_interp /\ init cond *)
+
+    -                                              
+          
+
+
+      admit.
+
+    - t.
+
+      + lazymatch goal with
+        | [ |- match result_bind (bool_result ?x) _ with _ => _ end] =>
+          destruct x eqn:?; cbn; ceauto
+        end.
+
+        t.
+
+        * admit. (* getEnv and v *)
+        * admit. (* pure calculation *)
+        * admit. (* may_read0 true case *)
+        * admit. (* may_read0 false case *)
+
+      + lazymatch goal with
+        | [ |- match result_bind (bool_result ?x) _ with _ => _ end] =>
+          destruct x eqn:?; cbn; ceauto
+        end.
+
+        destruct (latest_write0 (log ++ Log)) as [ [? ? ? ?] |] eqn:?; cbn.
+        replace (assert_size val (length l)) with (Success val) by admit. (* Log is consistent *)
+        cbn.
+        * t. (* latest_write0 *)
+          -- (* Lemma: constistent ⇒ latest_write0 ⇒ data0 is set *)
+            admit. (* FIXME: but this looks only at clog, not at CLog; why? *)
+          -- (* add_consistent *)
+            admit.
+          -- (* may_read1 ⇒ guard ok *)
+            admit.
+
+        * t. (* no latest write0 *)
+          -- consistent ⇒ latest_write0 none ⇒
+    - tstep.
+      tstep.
+      tstep.
+      tstep.
+      tstep.
+      tstep.
+      tstep.
+      tstep.
+      tstep.
+      tstep.
+      tstep.
+      tstep.
+      tstep.
+      tstep.
+      tstep.
+      tstep.
+      tstep.
+      tstep.
+      tstep.
+
+      match goal with
+      | [ H: retVal_consistent ?v ?bs |- context[?bs] ] =>
+        rewrite H
+      end.
+      tstep.
+      eauto.
+      tstep.
+      rewrite H2.
+      tstep.
+      tstep.
+      tstep.
+      tstep.
+      tstep.
+
+      lazymatch goal with
+      end.
+      eapply H; eassumption.
+      eapply (and_snd (and_snd H)).
+      intuition ceauto.
+
+    - tstep; ceauto.
+      tstep; ceauto.
+      tstep; ceauto.
+      tstep; ceauto.
+      tstep; ceauto.
+      2: admit.                 (* cond cannot run *)
+      tstep; ceauto.
+      tstep; ceauto.
+      tstep; ceauto.
+      tstep; ceauto.
+      tstep; ceauto.
+      tstep; ceauto.
+      2: admit.                (* Second branch of if *)
+      tstep; ceauto.
+      tstep; ceauto.
+      tstep; ceauto.
+      tstep; ceauto.
+      tstep; ceauto.
+      tstep; ceauto.
+      tstep; ceauto.
+
+    -
+
+    repeat match goal with
+           | _ => progress t
+           end.
+
+    repeat match goal with
+           end.
+    ceauto.
+
+    erewrite H1.
+    - cbn; intros.
+      destruct getenv eqn:?; cbn; ceauto; [].
+      intros.
+      destruct (getenv Gamma var); cbn; [ | admit (* would be inconsistent with gamma *) ].
+      ceauto. (* Just neet to have Some -> Some in the gammas here *)
+    - cbn; intros.
+      ceauto.
+    - cbn; intros.
+      ceauto.
+    - cbn; intros.
+
+      
